src/cddl/pulse/CDDL.Pulse.Serialize.Gen.MapGroup.ZeroOrMore.Aux2.fst
@@ -63,6 +63,9 @@ fn impl_serialize_map_zero_or_more_iterator_gen
   assert pure (cbor_parse_map_prefix_prop' p (U64.v count0) w0 (Seq.slice w0 0 (SZ.v size0)));
   let gmin = GR.alloc (0 <: nat);
   let gmax = GR.alloc (Some 0 <: option nat);
+  assume pure (
+    impl_serialize_map_zero_or_more_iterator_gen_invariant p em0 out w0 size0 count0 l v0 true
+  );
   while (
     !pres && not !pem
   )
@@ -85,6 +88,7 @@ fn impl_serialize_map_zero_or_more_iterator_gen
     let count = !out_count;
     if (count = pow2_64_m1) {
       pres := false;
+      assume pure False
     } else {
       let count' = U64.add count 1uL;
       S.pts_to_len out;
@@ -115,6 +119,7 @@ fn impl_serialize_map_zero_or_more_iterator_gen
         Pulse.Lib.Slice.join _ _ _;
         Trade.elim_hyp_l _ _ _;
         pres := false;
+        assume pure False
       } else {
         with w_out1 . assert (pts_to out1 w_out1);
         impl_serialize_parse_some minl maxl sp1 gk w_out1 size1;
@@ -130,6 +135,7 @@ fn impl_serialize_map_zero_or_more_iterator_gen
           Pulse.Lib.Slice.join _ _ out1;
           Pulse.Lib.Slice.join _ _ _;
           pres := false;
+          assume pure False
         } else {
           let ock = parse out1';
           let Some ck_ = ock;
@@ -162,6 +168,7 @@ fn impl_serialize_map_zero_or_more_iterator_gen
           S.pts_to_len out;
           if (ex) {
             pres := false;
+            assume pure False
           } else {
             let size1' = SZ.add size0 size1;
             let size2' = SZ.add size1' size2;
